added version 0.1 of crushEquality. proved eq dec for all types. excpet functions. need to work on that. going through other proofs now.

ProtoSynthDataTypes.v
@@ -1,29 +1,43 @@
-Add LoadPath "/users/paulkline/Documents/coqs/protosynth". 
+Add LoadPath "/users/paulkline/Documents/coqs/protosynth".
+Add LoadPath "/home/paul/Documents/coqs/protosynth/cpdt/src" as Cpdt.  
 Require Import MyShortHand.
 
 Inductive Noun : Set:=
   | VirusChecker
   | PCR.
-
+Theorem eq_dec_Noun : equality Noun.
+crush_equal. 
+Defined. 
+Hint Resolve eq_dec_Noun : eq_dec_db. 
 (* Now we define what it is we would like to know about these nouns. *)
 Inductive Attribute : Set :=
   | Name : Attribute
   | Hash : Attribute
   | Index : nat -> Attribute
   | Version : Attribute.
-
+Theorem eq_dec_Attribute : equality Attribute. 
+crush_equal. Defined. 
+Hint Resolve eq_dec_Attribute : eq_dec_db. 
 (*We only want to disallow nonsensical combinations, like a (PCR, version),
  hence this relation. *)
 Inductive DescriptionR : Noun -> Attribute -> Set :=
   | pcrMR : forall n, DescriptionR PCR (Index n)
   | virusCheckerNameR : DescriptionR VirusChecker Name
   | virusCheckerVersionR : DescriptionR VirusChecker Version.
-
+Theorem eq_dec_DescriptionR {n} {a}:  equality (DescriptionR n a).
+crush_equal. 
+Defined.
+Hint Resolve eq_dec_DescriptionR : eq_dec_db.  
+Hint Resolve eq_dec_DescriptionR.
+ 
 (* This 'extra step' is done simply so that comparison between descriptors
 is 'easy.'It is much more involved to be able to compare indexed types. *)
 Inductive Description : Set :=
   | descriptor {n : Noun} {a : Attribute} : DescriptionR n a -> Description.
-
+Theorem eq_dec_Description : equality Description.
+crush_equal. 
+Defined.
+Hint Resolve eq_dec_Description : eq_dec_db. 
 
 (*This defines what the type of measuring these things should be. *)
 Definition measurementDenote (d: Description) :=
@@ -39,6 +53,18 @@ end.
    but I want it to be certain values. *) 
 Inductive Requirement (d : Description) :=
 | requirement : ( (measurementDenote d) -> bool) -> Requirement d.
+Require Import FunctionalExtensionality. 
+Theorem eq_dec_f {A} {B} : forall (a b : (A -> B)), a =<> b.
+Proof. intros. Admitted.
+Hint Resolve eq_dec_f : eq_dec_db. 
+Theorem eq_dec_Requirement : forall d (x y : Requirement d), x =<> y.
+Proof. intros. 
+destruct d. 
+destruct d; 
+crush_equal. 
+Defined. 
+Hint Resolve eq_dec_Requirement : eq_dec_db.
+
 
 
 (* This begins the defining of what a privacy policy is. First we define a rule.
@@ -55,27 +81,95 @@ Inductive Rule (mything : Description) :=
 | never : Rule mything
 | multiReqAnd : Rule mything ->Rule mything -> Rule mything
 | multiReqOr : Rule mything -> Rule mything -> Rule mything.
+Theorem eq_dec_Rule : forall x, equality (Rule x).
+Proof.   intros.   intro_equals. 
+destruct x.  
+destruct d;
+generalize dependent x0; 
+induction y;
+intro_equals; 
+destruct x0; try first [decidable |  
+crush_equal].
+specialize IHy1 with x0_1. 
+specialize IHy2 with x0_2.
+destruct IHy1.  subst. 
+destruct IHy2.  subst. decidable. 
+decidable.  decidable.
+specialize IHy1 with x0_1. 
+specialize IHy2 with x0_2.
+destruct IHy1.  subst. 
+destruct IHy2.  subst. decidable.
+crush_equal. decidable.
+specialize IHy1 with x0_1. 
+specialize IHy2 with x0_2.
+destruct IHy1.  subst. 
+destruct IHy2.  subst. decidable. 
+decidable.  decidable.
+specialize IHy1 with x0_1. 
+specialize IHy2 with x0_2.
+destruct IHy1.  subst. 
+destruct IHy2.  subst. decidable.
+crush_equal. decidable.
 
+specialize IHy1 with x0_1. 
+specialize IHy2 with x0_2.
+destruct IHy1.  subst. 
+destruct IHy2.  subst. decidable. 
+decidable.  decidable.
+specialize IHy1 with x0_1. 
+specialize IHy2 with x0_2.
+destruct IHy1.  subst. 
+destruct IHy2.  subst. decidable.
+crush_equal. decidable.
+Defined.
+Hint Resolve eq_dec_Rule : eq_dec_db. 
 (* simply a list of rules. *)
 Inductive PrivacyPolicy :=
 | EmptyPolicy : PrivacyPolicy
 | ConsPolicy {d :Description}: 
     Rule d -> 
     PrivacyPolicy -> PrivacyPolicy.
-
+Theorem eq_dec_PrivacyPolicy : equality PrivacyPolicy.
+intro_equals.
+generalize dependent x. 
+induction y; try
+crush_equal + decidable.
+intros. destruct x; decidable.
+intros. destruct x. decidable. 
+ specialize IHy with x.
+ destruct IHy.  subst. crush_equal.  
+ crush_equal.
+Defined.
+Hint Resolve eq_dec_PrivacyPolicy : eq_dec_db. 
 Inductive Action : Set :=
  | ASend : Action
  | AReceive : Action.
-
+Theorem eq_dec_Action : equality Action. 
+crush_equal. 
+Defined.
+Hint Resolve eq_dec_Action : eq_dec_db. 
 (*A RequestItem is used to compose a list of the items and requirements upon 
 those items in an attestation *)
 Inductive RequestItem : Set :=
  | requestItem (d : Description) : (Requirement d) -> RequestItem.
-
+Theorem eq_dec_RequestItem : equality RequestItem.
+intro_equals.
+generalize dependent x.
+induction y;  intros. destruct x; try crush_equal.
+Defined.
+Hint Resolve eq_dec_RequestItem : eq_dec_db.
+ 
 Inductive RequestLS : Set :=
  | emptyRequestLS : RequestLS
  | ConsRequestLS : RequestItem -> RequestLS -> RequestLS.
+Theorem eq_dec_RequestLS : equality RequestLS.
+crush_equal. 
+Defined.
+Hint Resolve eq_dec_RequestLS : eq_dec_db.   
 
 Inductive Role : Set :=
  | Appraiser
  | Attester.
+Theorem eq_dec_Role : equality Role. 
+crush_equal. 
+Defined. 
