CrushEquality.v
@@ -1,0 +1,156 @@
+Require Import Coq.Classes.EquivDec.
+Require Export Coq.Program.Equality.
+Require Export Eqdep_dec.
+ 
+ Create HintDb eq_dec_db. 
+(**
+IMPORTANT:
+You MUST add each proof of equality to the eq_dec_db database
+(Hint Resolve <lemma_name> : eq_dec_db.)
+*)
+
+(** 
+We're going to be writing this a lot, so let's short hand it.
+*)
+Notation "x =<> y" := ({x = y} + {x <> y}) (at level 100).
+
+(** 
+We define a short hand for equality
+*)
+Definition equality (A :Type) := forall x y : A, x =<> y.  
+Hint Unfold equality : unfoldEq.
+
+Lemma eqNotation : forall A, (forall x y : A, (x =<> y)) -> (equality A).
+Proof. intro. autounfold with unfoldEq. intros.  auto.
+Defined.
+Hint Resolve eqNotation : eq_dec_db.
+   
+Lemma eqNotation2 : forall A, (equality A) ->  (forall x y : A, (x =<> y)) .
+Proof. intro. autounfold with unfoldEq. intros.  auto.
+Defined.
+Hint Resolve eqNotation2 : eq_dec_db.
+(** 
+The above was soooo necessary for proving x =<> y. otherwise auto can't figure out matching goal for it because it's stupid. Try 
+Print HintDb eq_dec_db to see that otherwise it doesn't work properly.*)
+
+
+(*  Ltac rec_eq :=
+ match goal with
+    | [ x : ?T, y : ?T |- _ ] => 
+       (match T with
+        | nat => generalize nat_eq_eqdec
+        | bool => generalize bool_eqdec
+        | unit => generalize unit_eqdec
+       end) ; 
+       intros X; destruct X with x y as [| paul];
+       try (left; inversion e; subst; reflexivity);
+       try (right; unfold complement in paul; unfold not; 
+            intros Hpaul; apply paul; inversion Hpaul; reflexivity)
+    end.
+
+Ltac eqdecHelper := subst; (left; reflexivity) || (
+right; unfold not; intros; inversion H; contradiction).
+ *)
+(**
+This will eliminate an existT in a Hypothesis.
+*)
+Ltac kill_existT' := match goal with 
+ | [ H : context[existT] |- _ ] => apply inj_pair2_eq_dec in H
+end.
+
+(** 
+Why is this next bit necessary you ask? Not sure, but repeat hangs forever. Therefore we use 'do' instead and apply kill existT' at most 5 times.\
+*) 
+Ltac kill_existT := first [ do 5 kill_existT' 
+                          | do 4 kill_existT' 
+                          | do 3 kill_existT' 
+                          | do 2  kill_existT' 
+                          | kill_existT']. 
+(**
+This helps us solve the case of not equals.
+*)
+Ltac not_eq := let nm1 := fresh "nEq" in (let nm2 := fresh "nEq" in  ((try right); unfold not; intros nm1; inversion nm1 as [nm2];
+     (try kill_existT); auto with eq_dec_db)).
+     
+
+Tactic Notation "intro_equals" := intros; autounfold with unfoldEq; intros.
+ Ltac eq_dec' name x y := assert (x =<> y) as name; auto with eq_dec_db.     
+Ltac dep_destruct_equality' name T := intro_equals;
+ match goal with 
+ | [ X : T,
+     Y : T |- _] => eq_dec' name X Y end.
+Ltac dep_destruct_equality name := intro_equals;
+ match goal with 
+ | [ x : ?X,
+     y : ?X
+       |- _ =<> _ ] => match goal with 
+           | [ H : x =<> y |- _] => fail 1
+           | _ =>  dep_destruct_equality' name X
+           end 
+       end.
+
+Add LoadPath "/home/paul/Documents/coqs/protosynth/cpdt/src" as Cpdt.
+Require Import Cpdt.CpdtTactics.
+Tactic Notation "depEqualSolver" := (match goal with 
+ | [x : ?T,
+    y : ?T
+          |- _ ] => (match goal with 
+                   | [ |- x =<> y ] => destruct x, y
+                   | _ => idtac "no need for pre-destruction"
+                  end); repeat (let nm := fresh "name" in 
+                     (dep_destruct_equality nm; 
+                      dep_destruct nm; subst; auto with eq_dec_db) 
+                   ); try not_eq
+ | _ => fail "no two same types in assumptions"
+ end).
+ 
+Ltac jmeq := match goal with 
+ [ H : ?T1 ~= ?T2 |- _] => apply JMeq_eq in H; auto
+ end. 
+Ltac jmeq_more := match goal with 
+ [ jmeq : ?T1 ~= ?T2 |- {?x = ?T2} + {?x <> ?T2} ] => apply JMeq_eq in jmeq;auto
+ end.
+
+Ltac destruct_equality := intro_equals; match goal with 
+ [ x : ?T,
+   y : ?T |- _] => destruct (equality T)
+   end.  
+   
+Ltac case_equals' name:= match goal with 
+ [ x : ?T,
+   y : ?T |- _] =>  assert ({x = y} + {x <> y}) as name; auto with *
+ end. 
+Tactic Notation "case_equals" := let name := fresh "equals" in case_equals' name.
+Tactic Notation "no" := (unfold not; let nm := fresh "H" in intro nm; inversion nm).
+ 
+Ltac dep_equal := intro_equals;
+match goal with 
+ [ x : ?T,
+   y : ?T |- {?x = ?y} + {?x <> ?y} ] => dep_destruct x; dep_destruct y;
+   (try (let eqName := fresh "equals" in (case_equals' eqName; destruct eqName))) ;
+   (solve  [(left; subst; auto)| right; no; auto]) + jmeq + idtac "jmeq tactic failed. Destruct so that your types match!"
+    
+ end. 
+
+Tactic Notation "decidable" := solve [(left; subst; auto)| right; no; auto]. 
+Tactic Notation "crush_equal" := 
+intro_equals; 
+try decide equality;
+solve [depEqualSolver; (decidable + not_eq) |  dep_equal; (decidable + not_eq)].
+
+Theorem eq_dec_List : forall A, equality A -> equality (list A). 
+Proof.  crush_equal. 
+Defined. 
+Hint Resolve eq_dec_List : eq_dec_db. 
+
+Theorem eq_dec_Pair : forall A B, equality A -> equality B -> equality (A*B). 
+crush_equal. 
+Defined. 
+Hint Resolve eq_dec_Pair : eq_dec_db. 
+
+Theorem eq_dec_ListPair : forall A B, equality A -> equality B -> equality (list(A*B)).
+crush_equal. 
+Defined. 
+Hint Resolve eq_dec_ListPair : eq_dec_db. 
+
+
