MyShortHand.v
@@ -5,27 +5,7 @@
 here are some comments
  *)
  
- Require Import Coq.Classes.EquivDec.
  
-Notation "x =<> y" := ({x = y} + {x <> y}) (at level 100).
- 
- Ltac rec_eq :=
- match goal with
-    | [ x : ?T, y : ?T |- _ ] => 
-       (match T with
-        | nat => generalize nat_eq_eqdec
-        | bool => generalize bool_eqdec
-        | unit => generalize unit_eqdec
-       end) ; 
-       intros X; destruct X with x y as [| paul];
-       try (left; inversion e; subst; reflexivity);
-       try (right; unfold complement in paul; unfold not; 
-            intros Hpaul; apply paul; inversion Hpaul; reflexivity)
-    end.
-
-Ltac eqdecHelper := subst; (left; reflexivity) || (
-right; unfold not; intros; inversion H; contradiction).
-
 Tactic Notation "inv" hyp(H) := inversion H; subst.
 Tactic Notation "cca" := repeat constructor; assumption.
 Tactic Notation "nono" := unfold not; let nm := fresh "X" in intro nm; inversion nm.
@@ -33,10 +13,13 @@ Tactic Notation "nono" hyp(H) :=  unfold not in H; exfalso; apply H; auto.
 Require Export Coq.Program.Equality.
 Require Export Eqdep_dec.
 Require Export Coq.Arith.EqNat.
-Require Export Coq.Arith.Peano_dec.
+Add LoadPath "/home/paul/Documents/coqs/protosynth".
+Add LoadPath "/home/paul/Documents/coqs/protosynth/cpdt/src" as Cpdt.   
+Require Export CrushEquality. 
+(* Require Export Coq.Arith.Peano_dec.
+ *)
 
-Ltac not_eq := let x := fresh "beats" in (let y := fresh "beats" in  ((try right); unfold not; intros x; inversion x as [y];
-     (try (apply inj_pair2_eq_dec in y); auto with eq_dec_db)  )). 
+ 
  (*
  knowing that a lower level binds more than a higher level. Hence the level for disjunction must be higher than the level for conjunction.
  Coq < Notation "A /\ B" := (and A B) (at level 80, right associativity).
@@ -56,8 +39,6 @@ Tactic Notation "gd" tactic (c) := generalize dependent c.
 Tactic Notation "s" := simpl. 
 Tactic Notation "s" ident (c) := simpl in c.
 Tactic Notation "c" := constructor. 
-
-
  
 Require Export String. Open Scope string_scope.
 Ltac move_to_top x :=
@@ -84,6 +65,46 @@ Tactic Notation "SSSSCase" constr(name) := Case_aux SSSSCase name.
 Tactic Notation "SSSSSCase" constr(name) := Case_aux SSSSSCase name.
 Tactic Notation "SSSSSSCase" constr(name) := Case_aux SSSSSSCase name.
 Tactic Notation "SSSSSSSCase" constr(name) := Case_aux SSSSSSSCase name.
+Add LoadPath "/home/paul/Documents/coqs/protosynth/cpdt/src" as Cpdt.
+Require Import Cpdt.CpdtTactics.
 
-(* ident string *)
+Definition xor (A : Prop) (B: Prop) := (A \/ B) /\ ~(A /\ B).
+
+
+
+(** proof command that aids in simple proofs of equality.
+ *)
+Ltac equal := autounfold with unfoldEq; repeat decide equality.
+
+(** 
+Handy Ltac  for simplifying Hypothesis' since simpl doesn't do it.
+Note: it will fail if the hypothesis doesn't change.
+*)
+Ltac simpl_H :=
+ match goal with 
+  [ H : ?T |- _] => progress (autounfold in H; (simpl in H))
+  end.
+Ltac cbn_H :=
+ match goal with 
+  [ H : ?T |- _] => progress (autounfold with * in H ; (cbn in H))
+  end.
+  
+(** 
+The actual command to use in proofs.
+will continue to apply until it fails. 
+*)
+Tactic Notation "sh" := repeat simpl_H.
+Tactic Notation "simplAll" := sh; autounfold; simpl.
+Tactic Notation "refl" := reflexivity.
+
+
+ 
+
+(*
+ *)
+Ltac inversion_any' := match goal with 
+[H : ?x = ?y |- _] => progress ( inversion H)
+end.
+Ltac inversion_any := solve [(repeat inversion_any')]. 
+
  
