ProtoSynthProtocolDataTypes.v
@@ -1,4 +1,5 @@
 Add LoadPath "/users/paulkline/Documents/coqs/protosynth". 
+Add LoadPath "/home/paul/Documents/coqs/protosynth/cpdt/src" as Cpdt. 
 Require Import MyShortHand.
 Require Import ProtoSynthDataTypes.
 
@@ -6,15 +7,43 @@ Inductive VarID :=
  | receivedMESSAGE : VarID
  | toSendMESSAGE : VarID
  | variden : nat -> VarID.
+Theorem eq_dec_VarID : equality VarID. 
+crush_equal. 
+Defined.
+Hint Resolve eq_dec_VarID : eq_dec_db. 
 
 Inductive Const :=
  | constValue (d: Description) : (measurementDenote d) -> Const 
  | constRequest : Description -> Const
  | constStop : Const.
+Theorem eq_dec_Const : equality Const.
+intro_equals. 
+destruct x,y.
+dep_destruct_equality nm.
+destruct nm.  subst.
+dep_destruct_equality nm2.
+destruct d0; try crush_equal.
+destruct d; crush_equal.
+crush_equal. 
+crush_equal. 
+crush_equal.
+decidable. 
+decidable.
+crush_equal.  
+decidable.
+decidable. 
+decidable. 
+decidable.
+Defined. 
+Hint Resolve eq_dec_Const : eq_dec_db. 
 
 Inductive Term :=
  | variable : VarID -> Term
  | const : Const -> Term.
+Theorem eq_dec_Term : equality Term. 
+crush_equal. 
+Defined. 
+Hint Resolve eq_dec_Term : eq_dec_db. 
 
 Inductive Condition :=
  | IsMyTurntoSend : Condition
@@ -26,16 +55,28 @@ Inductive Condition :=
  | IsRequest : Term -> Condition
  | IsStop : Term -> Condition
  | IsAllGood : Condition.
+Theorem eq_dec_Condition : equality Condition. 
+crush_equal. 
+Defined. 
+Hint Resolve eq_dec_Condition : eq_dec_Condition. 
 
 Inductive AllGood :=
  | Yes
  | No
  | Unset.
+Theorem eq_dec_AllGood : equality AllGood. 
+crush_equal. 
+Defined. 
+Hint Resolve eq_dec_AllGood : eq_dec_db. 
 
 Inductive Computation := 
  | compGetMessageToSend
  | compGetNextRequest
  | compGetfstQueue.
+Theorem eq_dec_Computation : equality Computation. 
+crush_equal. 
+Defined. 
+Hint Resolve eq_dec_Computation : eq_dec_db. 
 
 Inductive Effect :=
  | effect_StoreRequest : Term -> Effect
@@ -45,11 +86,17 @@ Inductive Effect :=
  | effect_rmFstQueued : Effect
  | effect_cp_ppUnresolved : Term -> Effect
  | effect_setAllGood : AllGood -> Effect.
-
+Theorem eq_dec_Effect : equality Effect. 
+crush_equal. 
+Defined. 
+Hint Resolve eq_dec_Effect : eq_dec_db. 
 Inductive Participant :=
  | ATTESTER
  | APPRAISER.
-
+Theorem eq_dec_Participant : equality Participant. 
+crush_equal. 
+Defined. 
+Hint Resolve eq_dec_Participant : eq_dec_db. 
 Inductive Statement :=
  | SendStatement : Term -> Participant -> Participant -> Statement
  | ReceiveStatement : VarID -> Statement
@@ -62,24 +109,47 @@ Inductive Statement :=
  | EndStatement : Statement
  | Skip : Statement
  | Wait : Statement.
-
+Theorem eq_dec_Statement : equality Statement. 
+crush_equal. 
+Defined. 
+Hint Resolve eq_dec_Statement : eq_dec_Statement. 
 Notation "'IFS' x 'THEN' y 'ELSE' z" := (Choose x y z)(at level 80, right associativity). 
 Notation "x '>>' y" := (Chain x y)  (at level 60, right associativity).
 
 Definition VarState := list (VarID*Const).
+Theorem eq_dec_VarState : equality VarState. 
+crush_equal. 
+Defined.
+Hint Resolve eq_dec_VarState : eq_dec_db. 
  
 Inductive ProState :=
  (*  action <who am I?> privacyPol <things I want to ask for!> <Things I've asked for and am waiting for a response> tosend *)
  | proState : Action -> AllGood -> Participant ->  PrivacyPolicy -> RequestLS -> RequestLS -> list Description
       -> ProState.
+Theorem eq_dec_ProState : equality ProState.
+crush_equal. 
+Defined. 
+Hint Resolve eq_dec_ProState : eq_dec_db. 
       
 Inductive State :=
  state : VarState -> ProState -> State.
+Theorem eq_dec_State : equality State.
+crush_equal. 
+Defined. 
+Hint Resolve eq_dec_State : eq_dec_db. 
 
 Inductive NetworkMessage :=
- networkMessage : Participant -> Participant -> Const -> NetworkMessage. 
+ networkMessage : Participant -> Participant -> Const -> NetworkMessage.
+Theorem eq_dec_NetworkMessage : equality NetworkMessage.
+crush_equal. 
+Defined. 
+Hint Resolve eq_dec_NetworkMessage : eq_dec_db. 
+ 
 Definition Network := list NetworkMessage.
-
+Theorem eq_dec_Network : equality Network. 
+crush_equal. 
+Defined. 
+Hint Resolve eq_dec_Network : eq_dec_db. 
 
 Definition mkState (a : Action) (p : Participant) (pp : PrivacyPolicy) (rls : RequestLS) : State:=
  state nil (proState a Yes p pp rls emptyRequestLS nil).
