maker.sh
@@ -1,7 +1,6 @@
 #!/usr/bin/env bash
 rm *.vo
+coqc CrushEquality.v &&
 coqc MyShortHand.v &&
 coqc ProtoSynthDataTypes.v &&
-coqc ProtoSynthProtocolDataTypes.v &&
-coqc ProtoSynthDataTypeEqualities.v
-
+coqc ProtoSynthProtocolDataTypes.v
